examples/ghc/lib/Bag.v
@@ -43,6 +43,11 @@ Arguments UnitBag {_} _.
 Arguments TwoBags {_} _ _.
 
 Arguments ListBag {_} _.
+(* Midamble *)
+
+Instance Default_Bag {a} : GHC.Err.Default (Bag a):=
+  GHC.Err.Build_Default _ EmptyBag.
+
 (* Converted value declarations: *)
 
 (* Skipping instance Outputable__Bag of class Outputable *)
