examples/ghc/module-edits/Bag/midamble.v
@@ -1,0 +1,2 @@
+Instance Default_Bag {a} : GHC.Err.Default (Bag a):=
+  GHC.Err.Build_Default _ EmptyBag.
