examples/ghc/module-edits/UnVarGraph/midamble.v
@@ -1,3 +1,9 @@
+Instance Default_UnVarSet : GHC.Err.Default UnVarSet :=
+  GHC.Err.Build_Default _ (Mk_UnVarSet GHC.Err.default).
+Instance Default_UnVarGraph : GHC.Err.Default UnVarGraph :=
+  GHC.Err.Build_Default _ (Mk_UnVarGraph GHC.Err.default).
+
+
 Instance Unpeel_UnVarSet : Prim.Unpeel UnVarSet Data.IntSet.Internal.IntSet :=
   Prim.Build_Unpeel _ _ (fun x => match x with | Mk_UnVarSet y => y end) Mk_UnVarSet.
 Instance Unpeel_UnVarGraph : Prim.Unpeel UnVarGraph (Bag.Bag Gen) :=
